verification/proofs/Chunk_hexVal/obl_pre_ret2_1.lean
@@ -1,4 +1,4 @@
-  simp only [inv_17, inv_36, inv_55, inv_59]
+  simp only [inv_ret0, inv_ret1, inv_ret2, inv_ret3]
   simp [run, step, P, hpc, hstk, State.set, pLt, pGt, *] at hrun
   subst hrun
   simp only [State.set, Nat.reduceEqDiff, reduceIte]
